# 2.2 Currying

### Motivation

look again at the summation function

def sumInts(a: Int, b: Int) = sum(x =>x, a, b)

Note that a and b get passed unchanged from sumInts into sum

can we be even shorter by getting rid of these parameters?

### functions returning functions

lets rewrite sum as follows

def sum(f: Int => Int): (Int, Int) = > Int = {
    def sumF(a: Int, b: Int): Int =
      if (a > b) 0
      else f(a) + sumF(a+ 1, b)
    sumF
}

sum is now a function that returns another function

the return function sumF applies the given function parameter f and sums the results

 ### stepwise applications
 
 we can define:
 
 def sumInts = sum(x => x)
 def sumCube = sum(x => x * x * x)
 def sumFactorials = sum(fact)
 
 these functions can in turn be applied like any other function:
 
 sumCube(1, 10) + sumFactorials(10, 20)
 
 ### consecutive stepwise applications
 
 in the previous example, we avoid the sumInts, sumCubes, middlemen
 
 sum (cube) (1, 10)
 
- sum(cube) applies sum to cube and returns the sum of cubes function
- sum(cube) is therefore equivalent to sumCubes
- this function is next applied to arguments (1, 10)
 
generally, function application associates to the left:

sum(cube)(1, 10) == (sum (cube)) (1, 10)

### multiple parameter lists

the definitions of functions that return functions is so useful in functional programming that there is special syntax for it in Scala

for example, the following definition of sum is equivalent to the one with the nested sumF function, but sorter

def sum(fL Int => Int)(a: Int, b: Int): Int =
  if (a > b) 0 else f(a) + sum(f)(a + 1, b)
  
this allows you to define id, cube, or fact with no parameters

stopped at 4:30 